more

coq/aop/Rel.v
@@ -364,3 +364,37 @@ Proof.
           change ((prj2 ; s) x y) in H4. rewrite <- H2 in H4.
           unfold comp in H4. destruct H4 as [z [H4 H5]]. destruct H5. assumption.
 Qed.
+
+Inductive Void : Type :=.
+
+Notation "0" := (Void) : Rel_scope.
+
+Open Scope Rel_scope.
+
+Definition initial (a:Type) : R 0 a := fun x y => False.
+
+Arguments initial {a}.
+
+Definition terminal (a:Type) : R a 0 := fun x y => False.
+
+Arguments terminal {a}.
+
+Lemma initial_existence : forall (a:Type), exists (r:R 0 a), True.
+Proof.
+    intros a. exists initial. trivial.
+Qed.
+
+Lemma initial_uniqueness : forall (a:Type) (r s:R 0 a), r = s.
+Proof.
+    intros a r s. apply Ext. intros x y. split; intros H1; inversion x.
+Qed.
+
+Lemma terminal_existence : forall (a:Type), exists (r:R a 0), True.
+Proof.
+    intros a. exists terminal. trivial.
+Qed.
+
+Lemma terminal_uniqueness : forall (a:Type) (r s:R a 0), r = s.
+Proof.
+    intros a r s. apply Ext. intros x y. split; intros H1; inversion y.
+Qed.
