lean/while/Swap.lean
@@ -13,6 +13,8 @@ def p₂(n m:ℕ) : Pred := λ s, s "x" = m ∧ s "y" = n
 
 def p₃(n m:ℕ) : Pred := λ s, s "t" = n ∧ s "y" = m
 
+def p₄(n m:ℕ) : Pred := λ s, s "x" = m ∧ s "t" = n
+
 lemma L0 : "y" = "t" = false :=
 begin
   apply propext, split,
@@ -20,20 +22,43 @@ begin
     { intros H1, contradiction }
 end
 
+
 lemma L1 : ∀ (n m:ℕ), subst "t" x (p₃ n m) = p₁ n m :=
 begin
   intros n m,
   unfold subst, unfold bindVar, unfold p₁, unfold p₃,
   unfold x, unfold aVar,
-  apply funext, intros s, apply propext, split; intros H1,
-    { cases H1 with H1 H2, simp at H1, },
-    {}
+  apply funext, intros s, apply propext, split; intros H1; cases H1 with H1 H2,
+    { simp at H1, cases decidable.em ("y" = "t") with H3 H3,
+      { exfalso, revert H3, from dec_trivial},
+      { simp [H3] at H2, split; assumption }},
+    { split,
+      { simp, assumption },
+      { cases decidable.em ("y" = "t") with H3 H3,
+        { exfalso, revert H3, from dec_trivial },
+        { simp [H3], assumption }}}
 end
 
+lemma L2 : ∀ (n m:ℕ), subst "x" y (p₄ n m) = p₃ n m :=
+begin
+  intros n m,
+  unfold subst, unfold bindVar, unfold p₃, unfold p₄, unfold y, unfold aVar,
+  apply funext, intros s, apply propext, split; intros H1; cases H1 with H1 H2,
+    { simp at H1, cases decidable.em ("t" = "x") with H3 H3,
+      { exfalso, revert H3, from dec_trivial },
+      { simp [H3] at H2, split; assumption }},
+    {split,
+      { simp, assumption },
+      { cases decidable.em ("t" = "x") with H3 H3,
+        { exfalso, revert H3, from dec_trivial },
+        { simp [H3], assumption }}}
+end
 
 lemma Swap_Correct : ∀ (n m:ℕ), Hoare (p₁ n m) Swap (p₂ n m) :=
 begin
-  intros n m, unfold Swap, apply (seq_intro _ (λ s, s "t" = n ∧ s "y" = m)),
-    { },
-    {}
+  intros n m, unfold Swap, apply (seq_intro _ (p₃ n m)),
+    { rw ← L1, apply assign_intro },
+    { apply (seq_intro _ (p₄ n m)),
+      { rw ← L2, apply assign_intro },
+      {}}
 end
